proof/ConRon/Refine2.lean
@@ -39,3 +39,9 @@ import ConRon.Refine2.ExprOps.Mut
 import ConRon.Refine2.Checker.Shape
 import ConRon.Refine2.Promote.Intern
 import ConRon.Refine2.Promote.Promote
+import ConRon.Refine2.Checker.KnotHyp
+import ConRon.Refine2.Checker.Pins
+import ConRon.Refine2.Checker.Canon
+import ConRon.Refine2.Checker.Axioms
+import ConRon.Refine2.Checker.Spec
+import ConRon.Refine2.Checker.Base
